VeriSkel/Extract.v
@@ -1,4 +1,4 @@
-Require Import Compiler.
+Require Import Compiler Examples Ext.
 
 Require Import ExtrOcamlBasic ExtrOcamlBigIntConv ExtrOcamlIntConv ExtrOcamlNatBigInt
         ExtrOcamlNatInt  ExtrOcamlString ExtrOcamlZBigInt ExtrOcamlZInt.
@@ -8,6 +8,8 @@ Extraction Blacklist List String Int.
 (* Extract Inductive nat => int ["0" "succ"] "(\fO fS n -> if n == 0 then fO () else fS (n-1))". *)
 (* Extract Inductive prod => "(,)" ["(,)"]. *)
 
+Extract Constant save_to_file => "Printer.save_to_file".
+
 Cd "extracted".
 
-Separate Extraction Compiler.
+Separate Extraction Examples.
